add: extraction to certified checker

checker/bin/main.ml
@@ -1,0 +1,96 @@
+let print_certificate file sko =
+  let mk_line s =
+    let l = String.length s in
+    let st = 60 - (l / 2) in
+    let ed = 120 - st - l in
+    Printf.sprintf "│%s%s%s│" (String.make st ' ') file (String.make ed ' ') in
+  let file = mk_line file in
+  Printf.printf {|
+╔────────────────────────────────────────────────────────────────────────────────────────────────────────────────────────╗
+│                  _____          _   _  __ _           _                __   _____                  __                  │
+│                 / ____|        | | (_)/ _(_)         | |              / _| |  __ \                / _|                 │
+│                | |     ___ _ __| |_ _| |_ _  ___ __ _| |_ ___    ___ | |_  | |__) | __ ___   ___ | |_                  │
+│                | |    / _ \ '__| __| |  _| |/ __/ _` | __/ _ \  / _ \|  _| |  ___/ '__/ _ \ / _ \|  _|                 │
+│                | |___|  __/ |  | |_| | | | | (_| (_| | ||  __/ | (_) | |   | |   | | | (_) | (_) | |                   │
+│                 \_____\___|_|   \__|_|_| |_|\___\__,_|\__\___|  \___/|_|   |_|   |_|  \___/ \___/|_|                   │
+│                                                                                                                        │
+│                                                                                                                        │
+│          ______)                                                                                                       │
+│         (, /  /)                       ,  /) ,                  ,                          /)      /)                  │
+│           /  (/    _    _   _  __ _/_    //    _  _  _/_  _       _     _  _   _ _   __  _(/  _  _(/   _/_ ___ '       │
+│        ) /   / )__(/_  (___(/_/ (_(___(_/(__(_(__(_(_(___(/_  _(_/_)_  (_(_(_(/ (_(_/ (_(_(__(/_(_(_   (__(_)  '       │
+│       (_/                              /)                                                                              │
+│                                       (/                                                                               │
+│                                                                                                                        │
+│                                                                                                                        │
+%s
+│                                                                                                                        │
+│               for being a successful first-order tableau proof certificate in %s Skolemization.                     │
+│                                                                                                                        │
+│                                                                                                                        │
+│                                                                                                                        │
+│                                                                                                                        │
+│                8                                                   8""""8 8"""88 8   8 8     8"""" ""8""               │
+│                8  eeeee eeeee e   e eeee eeeee    eeeee  e    e    8    8 8    8 8   8 8     8       8                 │
+│                8e 8   " 8   " 8   8 8    8   8    8   8  8    8    8eeee8 8    8 8e  8 8e    8eeee   8e                │
+│                88 8eeee 8eeee 8e  8 8eee 8e  8    8eee8e 8eeee8    88     8    8 88  8 88    88      88                │
+│                88    88    88 88  8 88   88  8    88   8   88      88     8    8 88  8 88    88      88                │
+│                88 8ee88 8ee88 88ee8 88ee 88ee8    88eee8   88      88     8eeee8 88ee8 88eee 88eee   88                │
+│                                                                                                                        │
+╚────────────────────────────────────────────────────────────────────────────────────────────────────────────────────────╝|} file sko
+
+type sko = Outer | Inner
+
+let sko_str = function
+  | Outer -> "outer"
+  | Inner -> "inner"
+
+let interp_sko = function
+  | Outer -> Lib.SkolemizationInstances.coq_OuterSkolemization
+  | Inner -> Lib.SkolemizationInstances.coq_InnerSkolemization
+
+let main () =
+  let file = ref "" in
+  let sko = ref Outer in
+  let fancy = ref false in
+  let select_skolemization = function
+    | "inner" -> sko := Inner
+    | _ -> () in
+  let optlist =
+    [ ("-skolem", Arg.String select_skolemization, "Skolemization mode of the proof. Default: outer.")
+    ; ("-fancy", Arg.Set fancy, "Print a fancy certificate instead of a simple message on successful verification. Default: false.")
+    ] in
+  let msg = "Welcome to POULET, the PrOof-checker for tableaUx in first-order Logic Extracted from Tableauxrocq.\n" in
+  let _ = Arg.parse optlist (fun s -> file := s) msg in
+  let where_from = open_in !file in
+  let lexbuf = Lexing.from_channel where_from in
+  begin
+    try
+      let declarations = Lib.Parser.proof Lib.Lexer.token lexbuf in
+      let fs,sigma,ruletree = Lib.Grammar.interp_decl_list declarations in
+      let status,err = Lib.Checker.coq_CheckProof (interp_sko !sko) fs sigma ruletree in
+      if status then
+        ((if !fancy then print_certificate !file (sko_str !sko)
+          else Printf.printf "The file contains a valid tableau proof.");
+         exit 0)
+      else
+        Printf.printf "Proof checking has reported an error:\n\"%s\"\n" (Lib.Prelude.RocqStr.to_string (List.hd err))
+    with
+    | Lib.Grammar.MultipleSubEncountered ->
+       Printf.printf "Error: multiple declarations with the substitution role encountered.\n"
+    | Lib.Grammar.NoSuchName name ->
+       Printf.printf "Error: found reference to an unknown name \"%s\"." name
+    | Lib.Grammar.DefCycleFound path ->
+       Printf.printf "Error: cycle of dependencies between the definitions (%s).\n" (String.concat " -> " path)
+    | Lib.Grammar.ProofCycleFound path ->
+       Printf.printf "Error: cyclic proof encountered (%s).\n" (String.concat " -> " path)
+    | Lib.Grammar.MalformedProof reason ->
+       Printf.printf "Error. %s\n" reason
+    | Lib.Parser.Error ->
+       Printf.printf "Syntax error on line %d encountered on lexeme \"%s\"\n"
+         lexbuf.Lexing.lex_curr_p.pos_lnum
+         (Lexing.lexeme lexbuf)
+  end;
+  exit 1
+
+let _ = main ()
