checker/lib/grammar.ml
@@ -1,0 +1,370 @@
+open Prelude
+open SyntaxInstance
+open ProofInstance
+open LocallyNamelessClasses
+open ExtendedSyntax
+
+module Inference = struct
+  type rule =
+    False | NotTrue | Hyp | NotNot | And | NotOr | NotImplies | Or | Implies |
+    NotAnd | Iff | NotIff | Exists | NotAll | Forall | NotEx
+
+  type t = { rule: rule; children: string list; new_term: coq_ETerm option }
+
+  let mk rule children new_term =
+    { rule; children; new_term = new_term }
+end
+
+type sub = (string * coq_ETerm)
+let mk_sub name tm = (name, tm)
+
+module Decl = struct
+  type role = Axiom | Conj | NegConj | LocDef | ProofStep
+  type plain = { name: string; role: role; targets: coq_EForm list; inf: Inference.t option }
+  type t = Plain of plain | Subst of ((string * coq_ETerm) list)
+
+  let mk name role target inf =
+    Plain { name; role; targets = [target]; inf = Some inf }
+
+  let mk_def name role target =
+    Plain { name; role; targets = [target]; inf = None }
+
+  let mk_hyp name role targets inf =
+    Plain { name; role; targets; inf = Some inf }
+
+  let mk_sub sub = Subst sub
+end
+
+exception NoSuchName of string
+let list_assoc name assoc =
+  try List.assoc name assoc
+  with
+  | Not_found -> raise (NoSuchName name)
+
+let rec referenced_names f names =
+  match f with
+  | ETop | EBot -> []
+  | EPred (p, _) ->
+     let name = RocqStr.to_string p in
+     if List.mem name names then [name]
+     else []
+  | ENeg f | EEx (_, f) | EAll (_, f) -> referenced_names f names
+  | EOr (f, g) | EAnd (f, g) | EImp (f, g) | EEqu (f, g) ->
+     List.append (referenced_names f names) (referenced_names g names)
+
+exception CycleFound of string list
+
+let dfs vertices g visited s =
+  let rec explore path visited v =
+    if List.mem v path then raise (CycleFound path)
+    else if List.mem v visited then visited
+    else v :: List.fold_left (explore (v :: path)) visited (list_assoc v g) in
+  explore [] visited s
+
+let toposort vertices edges =
+  List.fold_left (fun visited v -> dfs vertices edges visited v) [] vertices
+
+exception DefCycleFound of string list
+
+(* Topological sort of the definitions.
+   There is an edge between two definitions whenever a definition refers to another one.
+   This way, a formula can be normalized by replacing the symbols in the order given by
+   the topological sort. *)
+let sort_normalization defs =
+  let open Decl in
+  let _ = List.iter (fun d -> assert (List.length d.targets = 1)) defs in
+  let vertices = List.map (fun d -> d.name) defs in
+  let edges = List.map (fun d -> (d.name, referenced_names (List.hd d.targets) vertices)) defs in
+  try
+    toposort vertices edges
+  with CycleFound path -> raise (DefCycleFound path)
+
+let normalize_form gamma defs f =
+  let rec normalize_aux name nf f =
+    match f with
+    | ETop | EBot -> f
+    | EPred (p, _) ->
+       if RocqStr.to_string p = name
+       then nf
+       else f
+    | ENeg f -> ENeg (normalize_aux name nf f)
+    | EOr (f, g) -> EOr (normalize_aux name nf f, normalize_aux name nf g)
+    | EAnd (f, g) -> EAnd (normalize_aux name nf f, normalize_aux name nf g)
+    | EImp (f, g) -> EImp (normalize_aux name nf f, normalize_aux name nf g)
+    | EEqu (f, g) -> EEqu (normalize_aux name nf f, normalize_aux name nf g)
+    | EAll (x, f) -> EAll (x,normalize_aux name nf f)
+    | EEx (x, f) -> EEx (x,normalize_aux name nf f) in
+  let get_nf name = List.hd ((List.hd (List.filter (fun d -> d.Decl.name = name) defs)).targets) in
+  List.fold_left (fun f name -> normalize_aux name (get_nf name) f) f gamma
+
+exception MultipleSubEncountered
+
+let rec mk_substitution = function
+  | None | Some [] -> fun x -> Syntax.Free x
+  | Some ((x, t) :: xs) ->
+     let sigma = mk_substitution (Some xs) in
+     fun y -> if x = RocqStr.to_string y then translate_ETerm [] t else sigma y
+
+let interp_form_list gamma defs fs =
+  let open Decl in
+  let rec interp_roles = function
+    | [] -> []
+    | x :: xs ->
+       assert (List.length x.targets = 1);
+       assert (x.inf = None);
+       (match x.role with
+       | Axiom | NegConj -> List.hd x.targets
+       | Conj -> ENeg (List.hd x.targets)
+       | _ -> assert false) :: interp_roles xs in
+  let fs = interp_roles fs in
+  let fs = List.map (normalize_form gamma defs) fs in
+  List.map translate_EForm fs
+
+type eRule =
+| ERNotNot of coq_EForm
+| ERAnd of coq_EForm
+| ERNotOr of coq_EForm
+| ERNotImplies of coq_EForm
+| EROr of coq_EForm
+| ERImplies of coq_EForm
+| ERNotAnd of coq_EForm
+| ERIff of coq_EForm
+| ERNotIff of coq_EForm
+| ERNotEx of coq_EForm * coq_ETerm
+| ERAll of coq_EForm * coq_ETerm
+| ERNotAll of coq_EForm * coq_ETerm
+| EREx of coq_EForm * coq_ETerm
+
+type eRuleTree =
+  | LeafNotTop | LeafBot
+  | LeafHyp of (coq_EForm * coq_EForm)
+  | Node of eRuleTree * eRule * eRuleTree
+
+let rec mk_etree gamma defs assoc step =
+  let open Decl in
+  let inf = Option.get step.inf in
+  let on_unary r =
+    assert (List.length step.targets = 1);
+    assert (List.length inf.children = 1);
+    let child = List.hd inf.children in
+    Node (mk_etree gamma defs assoc (list_assoc child assoc), r (List.hd step.targets), LeafBot) in
+  let on_binary r =
+    assert (List.length step.targets = 1);
+    assert (List.length inf.children = 2);
+    let child1 = List.hd inf.children in
+    let child2 = List.nth inf.children 1 in
+    Node (mk_etree gamma defs assoc (list_assoc child1 assoc),
+          r (List.hd step.targets), mk_etree gamma defs assoc (list_assoc child2 assoc)) in
+  let on_quant r =
+    assert (List.length step.targets = 1);
+    assert (List.length inf.children = 1);
+    assert (inf.new_term <> None);
+    let child = List.hd inf.children in
+    let tm = Option.get inf.new_term in
+    Node (mk_etree gamma defs assoc (list_assoc child assoc), r (List.hd step.targets) tm, LeafBot) in
+  match inf.rule with
+  | False -> LeafBot
+  | NotTrue -> LeafNotTop
+  | Hyp ->
+     assert (List.length step.targets = 2);
+     LeafHyp (List.hd step.targets, List.nth step.targets 1)
+  | NotNot -> on_unary (fun f -> ERNotNot (normalize_form gamma defs f))
+  | NotOr -> on_unary (fun f -> ERNotOr (normalize_form gamma defs f))
+  | And -> on_unary (fun f -> ERAnd (normalize_form gamma defs f))
+  | NotImplies -> on_unary (fun f -> ERNotImplies (normalize_form gamma defs f))
+  | Or -> on_binary (fun f -> EROr (normalize_form gamma defs f))
+  | Implies -> on_binary (fun f -> ERImplies (normalize_form gamma defs f))
+  | NotAnd -> on_binary (fun f -> ERNotAnd (normalize_form gamma defs f))
+  | Iff -> on_binary (fun f -> ERIff (normalize_form gamma defs f))
+  | NotIff -> on_binary (fun f -> ERNotIff (normalize_form gamma defs f))
+  | Exists -> on_quant (fun f tm -> EREx (normalize_form gamma defs f, tm))
+  | NotAll -> on_quant (fun f tm -> ERNotAll (normalize_form gamma defs f, tm))
+  | Forall -> on_quant (fun f tm -> ERAll (normalize_form gamma defs f, tm))
+  | NotEx -> on_quant (fun f tm -> ERNotEx (normalize_form gamma defs f, tm))
+
+exception MalformedProof of string
+let rec compile etree =
+  let open ProofInstance in
+  match etree with
+  | LeafBot -> Leaf None
+  | LeafNotTop -> Node (Leaf None, AlphaNegNeg (Syntax.Neg (Syntax.Neg Syntax.Bot)), Leaf None)
+  | LeafHyp (f, g) -> Leaf (Some (translate_EForm f, translate_EForm g))
+  | Node (left, rule, right) ->
+     match rule with
+     | ERNotNot f -> Node (compile left, AlphaNegNeg (translate_EForm f), Leaf None)
+     | ERNotOr  f -> Node (compile left, AlphaNegOr (translate_EForm f), Leaf None)
+     | EROr     f -> Node (compile left, BetaOr (translate_EForm f), compile right)
+     | ERAll (f, t) ->
+        begin
+          match t with
+          | EFun _ -> raise (MalformedProof "On rule forall: expected a variable, got a constant or a function.")
+          | EVar x -> Node (compile left, GammaAll (translate_EForm f, x), Leaf None)
+        end
+     | ERNotAll (f, t) -> Node (compile left, DeltaNegAll (translate_EForm f, translate_ETerm [] t), Leaf None)
+
+     | ERAnd f ->
+        (* [[ And f1 f2 ]] --> Neg (Or (Neg [[ f1 ]]) (Neg [[ f2 ]])) *)
+        let f1, f2 =
+          match f with
+          | EAnd (f1,f2) -> translate_EForm f1, translate_EForm f2
+          | _ -> raise (MalformedProof "On rule and: expected target formula to be a conjunction.") in
+        let f = translate_EForm f in
+        Node (Node (Node (compile left, AlphaNegNeg (Neg (Neg f2)), Leaf None),
+                    AlphaNegNeg (Neg (Neg f1)), Leaf None),
+              AlphaNegOr f, Leaf None)
+
+     | ERNotImplies f ->
+        (* [[ Neg (Imp f1 f2) ]] --> Neg (Or (Neg [[ f1 ]]) [[ f2 ]]) *)
+        let f = translate_EForm f in
+        let f1,f2 =
+          match f with
+          | Neg (Or (f1, f2)) -> f1,f2
+          | _ -> raise (MalformedProof "On rule notImp: expected target formula to be a negated implication.") in
+        Node (Node (compile left, AlphaNegNeg (Neg f1), Leaf None),
+              AlphaNegOr f, Leaf None)
+
+     | ERImplies f ->
+        (* [[ Imp f1 f2 ]] --> Or (Neg [[ f1 ]]) [[ f2 ]] *)
+        Node (compile left, BetaOr (translate_EForm f), Leaf None)
+
+     | ERNotAnd f ->
+        (* [[ Neg (And f1 f2) ]] --> Neg (Neg (Or (Neg [[ f1 ]]) (Neg [[ f2 ]]))) *)
+        let f = translate_EForm f in
+        let f' =
+          match f with
+          | (Neg (Neg f')) -> f'
+          | _ -> raise (MalformedProof "On rule notAnd: expected target formula to be a negated conjunction.") in
+        Node (Node (compile left, BetaOr f', compile right), AlphaNegNeg f, Leaf None)
+
+     | ERIff f ->
+        (* [[ Iff f1 f2 ]] = Neg (Or (Neg (Or (Neg [[ f1 ]]) [[ f2 ]])) (Neg (Or (Neg [[ f2 ]]) [[ f1 ]]))) *)
+        let f1,f2 =
+          match f with
+          | EEqu (f1, f2) -> f1,f2
+          | _ -> raise (MalformedProof "On rule iff: expected target formula to be an equivalence.") in
+        let f = translate_EForm f in
+        let f1' = translate_EForm f1 in
+        let f2' = translate_EForm f2 in
+        Node
+          ( Node
+              ( Node
+                  ( Node
+                      ( Node
+                          ( compile left
+                          , BetaOr (Or (Neg f2', f1'))
+                          , Leaf (Some (f1', Neg f1')))
+                      , BetaOr (Or (Neg f1', f2'))
+                      , Node
+                          ( Leaf (Some (f2', Neg f2'))
+                          , BetaOr (Or (Neg f2', f1'))
+                          , compile right))
+                  , AlphaNegNeg (Neg (Neg (Or (Neg f2', f1'))))
+                  , Leaf None)
+              , AlphaNegNeg (Neg (Neg (Or (Neg f1', f2'))))
+              , Leaf None)
+          , AlphaNegOr f
+          , Leaf None)
+
+     | ERNotIff f ->
+        (* [[ Not (Iff f1 f2) ]] = Neg (Neg (Or (Neg (Or (Neg [[ f1 ]]) [[ f2 ]])) (Neg (Or (Neg [[ f2 ]]) [[ f1 ]])))) *)
+        let f1,f2 =
+          match f with
+          | ENeg (EEqu (f1, f2)) -> f1,f2
+          | _ -> raise (MalformedProof "On rule notIff: expected target formula to be a negated equivalence.") in
+        let f = translate_EForm f in
+        let f' = match f with Neg (Neg f') -> f' | _ -> assert false in
+        let f1' = translate_EForm f1 in
+        let f2' = translate_EForm f2 in
+        Node
+          ( Node
+              ( Node
+                  ( Node
+                      ( compile left
+                      , AlphaNegNeg (Neg (Neg f1'))
+                      , Leaf None)
+                  , AlphaNegOr (Neg (Or (Neg f1', f2')))
+                  , Leaf None)
+              , BetaOr f'
+              , Node
+                  ( Node
+                      ( compile right
+                      , AlphaNegNeg (Neg (Neg f2'))
+                      , Leaf None)
+                  , AlphaNegOr (Neg (Or (Neg f2', f1')))
+                  , Leaf None))
+          , AlphaNegNeg f
+          , Leaf None)
+
+     | ERNotEx (f, t) ->
+        (* [[ Neg (Ex f) ]] = Neg (Neg (All (Neg [[ f ]]))) *)
+        let f = translate_EForm f in
+        let f' =
+          match f with
+          | Neg (Neg f') -> f' |
+          _ -> raise (MalformedProof "On rule notEx: expected target formula to be a negated existential.") in
+        let x =
+          match t with
+          | EFun _ -> raise (MalformedProof "On rule notEx: expected new term to be a variable.")
+          | EVar x -> x in
+        Node
+          ( Node
+              ( compile left
+              , GammaAll (f', x)
+              , Leaf None)
+          , AlphaNegNeg f
+          , Leaf None)
+
+     | EREx (f, t) ->
+        (* [[ Ex f ]] = Neg (All (Neg [[ f ]])) *)
+        let f = translate_EForm f in
+        let t = translate_ETerm [] t in
+        let g =
+          match f with
+          | Neg (All (Neg g)) ->
+             let atom = AtomInstances.string_atom in
+             varOpening (Syntax.opening_form atom atom atom) 0 t g
+          | _ -> raise (MalformedProof "On rule ex: expected target formula to be existential.") in
+        Node
+          ( Node
+              ( compile left
+              , AlphaNegNeg (Neg (Neg g))
+              , Leaf None)
+          , DeltaNegAll (f, t)
+          , Leaf None)
+
+exception ProofCycleFound of string list
+let interp_rules gamma defs tree =
+  let open Decl in
+  let get_children s = (Option.get s.inf).children in
+  let vertices = List.map (fun s -> s.name) tree in
+  let edges = List.map (fun s -> (s.name, get_children s)) tree in
+  let assoc = List.map (fun s -> (s.name, s)) tree in
+  try
+    let root = List.hd (toposort vertices edges) in
+    let etree = mk_etree gamma defs assoc (list_assoc root assoc) in
+    compile etree
+  with
+  | CycleFound path -> raise (ProofCycleFound path)
+
+let interp_decl_list ls =
+  let open Decl in
+  let rec interp_aux = function
+    | [] -> ([], [], None, [])
+    | x :: xs ->
+       let defs,fs,sub,tree = interp_aux xs in
+       match x with
+       | Decl.Subst sigma ->
+          if Option.is_some sub
+          then raise MultipleSubEncountered
+          else (defs,fs,Some sigma,tree)
+       | Decl.Plain step ->
+          match step.role with
+          | Axiom | Conj | NegConj -> defs,(step::fs),sub,tree
+          | LocDef -> step::defs,fs,sub,tree
+          | ProofStep -> defs,fs,sub,step::tree in
+  let defs,fs,sigma,tree = interp_aux ls in
+  let gamma = sort_normalization defs in
+  let fs = interp_form_list gamma defs fs in
+  let sigma = mk_substitution sigma in
+  let tree = interp_rules gamma defs tree in
+  fs,sigma,tree
