checker/lib/parser.mly
@@ -1,0 +1,205 @@
+%{
+
+	open Prelude
+	open Grammar
+	open ExtendedSyntax
+
+	let rec nest_all vs f =
+	  match vs with
+	  | [] -> f
+	  | x :: xs -> EAll (RocqStr.from_string x, nest_all xs f)
+
+	let rec nest_ex vs f =
+	  match vs with
+	  | [] -> f
+	  | v :: vs -> EEx (RocqStr.from_string v, nest_ex vs f)
+%}
+
+%token LPAR RPAR COMMA COLON DOT SEMI LBRACK RBRACK LACC RACC BACKQUOTE
+%token FOF PLAIN SUBST AXIOM CONJECTURE NEGATED_CONJECTURE DEFINITION TH LEM COR FOT INFERENCE
+%token LOR LAND LIMP LIFF LNEG LALL LEX FTRUE FFALSE ARR
+%token <int> INT
+%token <string> LOWER_WORD SQ_CHAR UPPER_WORD
+%token FALSE NOT_TRUE HYP NOT_NOT AND NOT_OR NOT_IMP OR IMP NOT_AND IFF NOT_IFF EX NOT_ALL ALL NOT_EX
+%token EOF
+
+%start proof
+
+%type <Decl.t list> proof
+
+%%
+
+proof:
+  decl_list EOF { $1 }
+;
+
+decl_list:
+    decl { [$1] }
+  | decl decl_list { $1 :: $2 }
+;
+
+decl:
+    fof_definition { $1 }
+  | fof_proof_step { $1 }
+  | fof_subst      { $1 }
+;
+
+fof_definition:
+  FOF LPAR name COMMA role COMMA fof_formula RPAR DOT { Decl.mk_def $3 $5 $7 }
+;
+
+fof_proof_step:
+    FOF LPAR name COMMA PLAIN COMMA fof_formula COMMA inference RPAR DOT { Decl.mk $3 Decl.ProofStep $7 $9 }
+  | FOF LPAR name COMMA PLAIN COMMA LBRACK RBRACK COMMA inference RPAR DOT { Decl.mk_hyp $3 Decl.ProofStep [] $10 }
+  | FOF LPAR name COMMA PLAIN COMMA LBRACK fof_formula_list RBRACK COMMA inference RPAR DOT { Decl.mk_hyp $3 Decl.ProofStep $8 $11 }
+;
+
+fof_subst:
+  FOF LPAR name COMMA SUBST COMMA LACC subst_list RACC RPAR DOT { Decl.mk_sub $8 }
+;
+
+name:
+    atomic_word { $1 }
+  | INT         { string_of_int $1 }
+;
+
+name_list:
+    name { [$1] }
+  | name COMMA name_list { $1 :: $3 }
+;
+
+role:
+    AXIOM { Decl.Axiom }
+  | TH { Decl.Axiom }
+  | LEM { Decl.Axiom }
+  | COR { Decl.Axiom }
+  | CONJECTURE { Decl.Conj }
+  | NEGATED_CONJECTURE { Decl.NegConj }
+  | DEFINITION { Decl.LocDef }
+;
+
+fof_formula:
+    fof_binary_formula { $1 }
+  | fof_unary_formula  { $1 }
+  | fof_unitary_formula  { $1 }
+;
+
+fof_formula_list:
+    fof_formula { [$1] }
+  | fof_formula COMMA fof_formula_list { $1 :: $3 }
+;
+
+inference:
+    INFERENCE LPAR rule COMMA LBRACK name_list RBRACK RPAR { Inference.mk $3 $6 None }
+  | INFERENCE LPAR rule COMMA LBRACK RBRACK RPAR { Inference.mk $3 [] None }
+  | INFERENCE LPAR rule COMMA LBRACK RBRACK COMMA FOT LPAR fof_term RPAR RPAR { Inference.mk $3 [] (Some $10) }
+  | INFERENCE LPAR rule COMMA LBRACK name_list RBRACK COMMA FOT LPAR fof_term RPAR RPAR { Inference.mk $3 $6 (Some $11) }
+;
+
+subst: UPPER_WORD ARR fof_term { mk_sub $1 $3 }
+;
+
+subst_list:
+    subst { [$1] }
+  | subst SEMI subst_list { $1 :: $3 }
+;
+
+rule:
+    FALSE { Inference.False }
+  | NOT_TRUE { Inference.NotTrue }
+  | HYP { Inference.Hyp }
+  | NOT_NOT { Inference.NotNot }
+  | AND { Inference.And }
+  | NOT_OR { Inference.NotOr }
+  | NOT_IMP { Inference.NotImplies }
+  | OR { Inference.Or }
+  | IMP { Inference.Implies }
+  | NOT_AND { Inference.NotAnd }
+  | IFF { Inference.Iff }
+  | NOT_IFF { Inference.NotIff }
+  | EX { Inference.Exists }
+  | NOT_ALL { Inference.NotAll }
+  | ALL { Inference.Forall }
+  | NOT_EX { Inference.NotEx }
+;
+
+fof_binary_formula:
+    fof_unit_formula LIFF fof_unit_formula { EEqu ($1, $3) }
+  | fof_binary_rightassoc { $1 }
+  | fof_binary_leftassoc { $1 }
+;
+
+fof_unary_formula: LNEG fof_unit_formula { ENeg $2 }
+;
+
+fof_unitary_formula:
+    fof_quantified_formula { $1 }
+  | fof_atomic_formula { $1 }
+  | LPAR fof_formula RPAR { $2 }
+;
+
+fof_binary_leftassoc:
+    fof_or_formula { $1 }
+  | fof_and_formula { $1 }
+;
+
+fof_binary_rightassoc: fof_imp_formula { $1 }
+;
+
+fof_unit_formula:
+    fof_unitary_formula { $1 }
+  | fof_unary_formula { $1 }
+;
+
+fof_or_formula:
+    fof_unit_formula LOR fof_unit_formula { EOr ($1, $3) }
+  | fof_or_formula LOR fof_unit_formula { EOr ($1, $3) }
+;
+
+fof_and_formula:
+    fof_unit_formula LAND fof_unit_formula { EAnd ($1, $3) }
+  | fof_or_formula LAND fof_unit_formula { EAnd ($1, $3) }
+;
+
+fof_imp_formula:
+    fof_unit_formula LIMP fof_unit_formula { EImp ($1, $3) }
+  | fof_unit_formula LIMP fof_imp_formula  { EImp ($1, $3) }
+;
+
+fof_quantified_formula:
+    LALL LBRACK fof_var_list RBRACK COLON fof_unit_formula { nest_all $3 $6 }
+  | LEX  LBRACK fof_var_list RBRACK COLON fof_unit_formula { nest_ex $3 $6  }
+;
+
+fof_atomic_formula:
+    atomic_word { EPred ((RocqStr.from_string $1), []) }
+  | atomic_word LPAR fof_arguments RPAR { EPred ((RocqStr.from_string $1), $3) }
+  | FTRUE { ETop }
+  | FFALSE { EBot }
+;
+
+fof_var_list:
+    UPPER_WORD { [$1] }
+  | UPPER_WORD COMMA fof_var_list { $1 :: $3 }
+;
+
+fof_arguments:
+    fof_term { [$1] }
+  | fof_term COMMA fof_arguments { $1 :: $3 }
+;
+
+fof_term:
+    fof_function_term { $1 }
+  | UPPER_WORD { EVar (RocqStr.from_string $1) }
+;
+
+fof_function_term:
+    atomic_word { EFun ((RocqStr.from_string $1), []) }
+  | atomic_word LPAR fof_arguments RPAR { EFun ((RocqStr.from_string $1), $3) }
+;
+
+atomic_word:
+    LOWER_WORD { $1 }
+  | SQ_CHAR { $1 }
+  | BACKQUOTE UPPER_WORD { $2 }
+;
