checker/lib/printer.ml
@@ -1,0 +1,25 @@
+open Syntax
+open SyntaxInstance
+
+let rec pr_form_ (pr_tm : coq_Term -> Prelude.RocqStr.t) f =
+  match f with
+  | Neg Bot -> "$true"
+  | Neg (Or (Neg (Or (Neg f, g)), Neg (Or (Neg g', f')))) when f = f' && g = g' ->
+     Printf.sprintf "(%s <=> %s)" (pr_form_ pr_tm f) (pr_form_ pr_tm g)
+  | Neg (Or (Neg f, Neg g)) -> Printf.sprintf "(%s & %s)" (pr_form_ pr_tm f) (pr_form_ pr_tm g)
+  | Or (Neg f, g) -> Printf.sprintf "(%s => %s)" (pr_form_ pr_tm f) (pr_form_ pr_tm g)
+  | Neg (All (Neg f)) -> Printf.sprintf "? (%s)" (pr_form_ pr_tm f)
+
+  | Bot -> "$false"
+  | Pred (p, ts) ->
+     Printf.sprintf "%s(%s)" (Prelude.RocqStr.to_string p) (String.concat ", " (List.map (fun t -> Prelude.RocqStr.to_string (pr_tm t)) ts))
+  | Neg f -> Printf.sprintf "~(%s)" (pr_form_ pr_tm f)
+  | Or (f, g) -> Printf.sprintf "(%s | %s)" (pr_form_ pr_tm f) (pr_form_ pr_tm g)
+  | All f -> Printf.sprintf "! (%s)" (pr_form_ pr_tm f)
+
+let pr_form pr_tm f = Prelude.RocqStr.from_string (pr_form_ pr_tm f)
+
+let pr_ctx_ (pr_tm : coq_Term -> Prelude.RocqStr.t) l =
+  Printf.sprintf "[\n\t%s\n]" @@ String.concat "\n\t" (List.map (pr_form_ pr_tm) l)
+
+let pr_ctx pr_tm l = Prelude.RocqStr.from_string (pr_ctx_ pr_tm l)
