checker/lib/printer.mli
@@ -1,0 +1,5 @@
+open SyntaxInstance
+
+val pr_form : (coq_Term -> Prelude.RocqStr.t) -> coq_Form -> Prelude.RocqStr.t
+
+val pr_ctx : (coq_Term -> Prelude.RocqStr.t) -> coq_Form list -> Prelude.RocqStr.t
