theories/Extraction.v
@@ -1,0 +1,47 @@
+From Tableaux Require Import Core.
+From Tableaux Require Import Checker.
+
+Extraction Language OCaml.
+Set Extraction Output Directory "../checker/lib/".
+
+(** ** Extraction for constants and basic inductives *)
+From Stdlib Require Import ExtrOcamlBasic.
+From Stdlib Require Export ExtrOcamlString.
+From Stdlib Require Import ExtrOcamlNatInt.
+
+Extract Inlined Constant map => "List.map".
+Extract Inlined Constant app => "List.append".
+Extract Inlined Constant rev => "List.rev".
+Extract Inlined Constant fold_left => "(fun f a l -> List.fold_left f l a)".
+Extract Inlined Constant fold_right => "(fun f a l -> List.fold_right f l a)".
+Extract Inlined Constant existsb => "List.exists".
+Extract Inlined Constant forallb => "List.for_all".
+Extract Inlined Constant filter => "List.filter".
+
+Extract Inlined Constant String.append => "List.append".
+
+Extract Inlined Constant fst => "fst".
+Extract Inlined Constant snd => "snd".
+
+Extract Inductive bool => bool [ "true" "false" ].
+Extract Inlined Constant negb => "Bool.not".
+
+Extraction Blacklist List String.
+
+(** ** Syntax *)
+Extract Inlined Constant eq_bool_string => "(=)".
+Extract Inlined Constant eq_bool_nat => "(=)".
+
+(** ** Checking *)
+Extract Inlined Constant pr_bool => "Bool.to_string".
+
+(** ** Extraction *)
+Extract Inlined Constant pr_form => "(Printer.pr_form pr_term)".
+Extract Inlined Constant Ctx.pr_ctx => "(Printer.pr_ctx pr_term)".
+
+Separate Extraction
+  ExtendedSyntax.translate_EForm
+  ProofInstance.RuleTree
+  SkolemizationInstances.OuterSkolemization
+  SkolemizationInstances.InnerSkolemization
+  Checker.CheckProof.
