theories/ProofInstance.v
@@ -1,0 +1,26 @@
+From Tableaux Require Import Prelude.All.
+From Tableaux Require Export Proofs.
+
+From Tableaux Require Export SyntaxInstance.
+From Tableaux Require Export SkolemizationInstances.
+
+Definition Tableau := @Tableau string string string _ _ _.
+
+(* XXX: This data structure should be shared with Tableaux.
+          We want a RuleTree and a TableauTree to coincide (actually, they almost already do so it should
+          be easy to unify them). *)
+
+(** We start by giving a data structure that reflects the rules of [ExpansionStep]. *)
+Inductive Rule : Type :=
+| AlphaNegNeg : Form -> Rule
+| AlphaNegOr : Form -> Rule
+| BetaOr : Form -> Rule
+| GammaAll : Form -> string -> Rule
+| DeltaNegAll : Form -> Term -> Rule.
+
+(** As we want a proof tree, we will take a tree of extended rules as an input of the algorithm.
+    Unary rules can be implemented by ignoring the _2nd_ child of the tree. *)
+Inductive RuleTree : Type :=
+| Leaf : option (Form * Form) -> RuleTree
+| Node : RuleTree -> Rule -> RuleTree -> RuleTree.
+
