theories/SkolemizationInstances.v
@@ -1,0 +1,7 @@
+From Tableaux Require Import Prelude.All.
+From Tableaux Require Export Skolemization.
+
+Definition Skolemization := Skolemization_ string string string.
+
+Definition OuterSkolemization : Skolemization := @OuterSkolemization string string string _ _ _ _.
+Definition InnerSkolemization : Skolemization := @InnerSkolemization string string string _ _ _ _.
