theories/SyntaxInstance.v
@@ -1,0 +1,410 @@
+(** * SyntaxInstance: instantiation of the atoms using strings *)
+
+From Tableaux Require Export Prelude.All.
+From Tableaux Require Export Syntax.
+
+From Stdlib Require Import Lia.
+From Stdlib Require Import Structures.Orders.
+
+Definition Term := Term string string.
+Definition Form := Form string string string.
+
+(** *** Sets of formulas *)
+
+(** We instantiate [MSetsAVL] with formulas to get sets of formulas. *)
+
+(** First, we add a propositional & boolean function to compare terms. *)
+Fixpoint lt_term (t u : Term) : Prop :=
+  match t, u with
+  | Bound n, Bound m => n < m
+  | Bound _, _ => True
+  | Free x, Free y => SOrd.lt x y
+  | Free _, Bound _ => False
+  | Free _, _ => True
+  | Fun f lf, Fun g lg =>
+      SOrd.lt f g \/
+        (f = g /\ lt_list lt_term lf lg)
+  | Fun _ _, _ => False
+  end.
+
+Fixpoint ltb_term (t u : Term) : bool :=
+  match t, u with
+  | Bound n, Bound m =>
+      match PeanoNat.Nat.compare n m with
+      | Lt => true
+      | _ => false
+      end
+  | Bound _, _ => true
+  | Free x, Free y =>
+      match SOrd.compare x y with
+      | Lt => true
+      | _ => false
+      end
+  | Free _, Bound _ => false
+  | Free _, _ => true
+  | Fun f lf, Fun g lg =>
+      match SOrd.compare f g with
+      | Lt => true
+      | Eq => ltb_list ltb_term lf lg
+      | Gt => false
+      end
+  | Fun _ _, _ => false
+  end.
+
+(** We have a reflection property on these two functions. *)
+Lemma ltb_term_lt_term :
+  forall (t u : Term),
+    ltb_term t u = true <-> lt_term t u.
+Proof.
+  intro t; induction t using term_ind; destruct u; try easy; cbn.
+  - destruct (PeanoNat.Nat.compare n n0) eqn:hcomp.
+    + apply PeanoNat.Nat.compare_eq in hcomp; subst.
+      split; intro contra.
+      * inversion contra.
+      * exfalso. now apply PeanoNat.Nat.lt_irrefl in contra.
+    + split; auto; intros _. now apply Compare_dec.nat_compare_Lt_lt.
+    + split; intro contra.
+      * inversion contra.
+      * exfalso. apply Compare_dec.nat_compare_Gt_gt in hcomp; lia.
+  - have hspec := SOrd.compare_spec a s.
+    destruct (SOrd.compare a s) eqn:hcomp.
+    + inversion hspec; subst; cbn in *.
+      split; intro contra.
+      * inversion contra.
+      * exfalso. now apply SOrd.lt_strorder in contra.
+    + inversion hspec; split; auto.
+    + inversion hspec; split; intro contra.
+      * inversion contra.
+      * exfalso. have hcontr : SOrd.lt s s.
+        { etransitivity; eauto. }
+        now apply SOrd.lt_strorder in hcontr.
+  - have hspec := SOrd.compare_spec f s.
+    destruct (SOrd.compare f s) eqn:hcomp.
+    + inversion hspec; subst. split; intro h.
+      * right; split; auto.
+        erewrite <-ltb_list_lt_list; eauto.
+        intros. eapply Ind.Forall_In in H; eauto.
+      * destruct h.
+        -- apply SOrd.lt_strorder in H0; auto.
+        -- destruct H0 as [_ hlt].
+           erewrite ltb_list_lt_list; eauto.
+           intros; eapply Ind.Forall_In in H; eauto.
+    + inversion hspec; split; auto.
+    + inversion hspec; split.
+      * intro contra; inversion contra.
+      * intros [ hlt | [e hlt] ].
+        -- have hlt' : SOrd.lt s s by etransitivity; eauto.
+           now apply SOrd.lt_strorder in hlt'.
+        -- subst. rewrite SSet.XOrdProps.ME.compare_refl in hcomp; inversion hcomp.
+Qed.
+
+Lemma ltb_term_false :
+  forall (t u : Term),
+    ltb_term t u = false -> t <> u -> ltb_term u t = true.
+Proof.
+  intro t; induction t using term_ind; intros ? hnlt ne; destruct u; cbn in *; try easy.
+  - have hspec := NOrd.compare_spec n n0.
+    destruct (PeanoNat.Nat.compare n n0); inversion hspec; try easy;
+      destruct (PeanoNat.Nat.compare n0 n) eqn:hcomp; try easy.
+    + exfalso; apply ne; now subst.
+    + apply Compare_dec.nat_compare_Gt_gt in hcomp; lia.
+    + apply PeanoNat.Nat.compare_eq in hcomp; lia.
+    + apply Compare_dec.nat_compare_Gt_gt in hcomp; lia.
+  - have hspec := SOrd.compare_spec a s.
+    destruct (SOrd.compare a s); inversion hspec; try easy;
+      destruct (SOrd.compare s a) eqn:hcomp; try easy.
+    + exfalso; apply ne; now subst.
+    + rewrite SSet.Raw.MX.compare_gt_iff in hcomp; subst.
+      now apply SOrd.lt_strorder in hcomp.
+    + apply SSet.Raw.MX.compare_eq in hcomp; subst.
+      exfalso; now apply ne.
+    + rewrite SSet.Raw.MX.compare_gt_iff in hcomp.
+      have contra : SOrd.lt s s by etransitivity; eauto.
+      now apply SOrd.lt_strorder in contra.
+  - have hspec := SOrd.compare_spec f s.
+    destruct (SOrd.compare f s); inversion hspec; try easy;
+      destruct (SOrd.compare s f) eqn:hcomp; try easy.
+    + subst. have ne' : l <> l0.
+      { intro; apply ne; now subst. }
+      apply ltb_list_false; auto.
+      intros; eapply Forall_In in H; eauto.
+    + subst. rewrite SSet.Raw.MX.compare_refl in hcomp. inversion hcomp.
+    + apply SSet.Raw.MX.compare_eq in hcomp; subst.
+      now apply SOrd.lt_strorder in H0.
+    + rewrite SSet.Raw.MX.compare_gt_iff in hcomp.
+      have contra : SOrd.lt s s by etransitivity; eauto.
+      now apply SOrd.lt_strorder in contra.
+Qed.
+
+(** We do the same for formulas. *)
+Fixpoint lt_form (F G : Form) : Prop :=
+  match F, G with
+  | Bot, Bot => False
+  | Bot, _ => True
+  | _, Bot => False
+
+  | Pred p l, Pred p' l' =>
+      SOrd.lt p p' \/
+        (p = p' /\ lt_list lt_term l l')
+  | Pred _ _, _ => True
+
+  | Neg F, Neg G => lt_form F G
+  | Neg _, Pred _ _ => False
+  | Neg _, _ => True
+
+  | Or F1 F2, Or G1 G2 =>
+      lt_form F1 G1 \/ (F1 = G1 /\ lt_form F2 G2)
+  | Or _ _, All _ => True
+  | Or _ _, _ => False
+
+  | All F, All G => lt_form F G
+  | All _, _ => False
+  end.
+
+Fixpoint ltb_form (F G : Form) : bool :=
+  match F, G with
+  | Bot, Bot => false
+  | Bot, _ => true
+  | _, Bot => false
+
+  | Pred p l, Pred p' l' =>
+      match SOrd.compare p p' with
+      | Lt => true
+      | Eq => ltb_list ltb_term l l'
+      | Gt => false
+      end
+  | Pred _ _, _ => true
+
+  | Neg F, Neg G => ltb_form F G
+  | Neg _, Pred _ _ => false
+  | Neg _, _ => true
+
+  | Or F1 F2, Or G1 G2 =>
+      ltb_form F1 G1 || (eqb F1 G1 && ltb_form F2 G2)
+  | Or _ _, All _ => true
+  | Or _ _, _ => false
+
+  | All F, All G => ltb_form F G
+  | All _, _ => false
+  end.
+
+Lemma ltb_form_lt_form :
+  forall (F G : Form),
+    ltb_form F G = true <-> lt_form F G.
+Proof.
+  intro F; induction F; intro G; destruct G; try easy; cbn.
+  - have hspec := SOrd.compare_spec p s.
+    destruct (SOrd.compare p s); inversion hspec.
+    + subst; split.
+      * intro hltb. right; split; auto.
+        rewrite -ltb_list_lt_list; eauto.
+        intros; apply ltb_term_lt_term.
+      * intros [ contra | [ _ hlt ] ].
+        -- now apply SOrd.lt_strorder in contra.
+        -- rewrite ltb_list_lt_list; eauto.
+           intros; apply ltb_term_lt_term.
+    + split; auto.
+    + split.
+      * intro contra; inversion contra.
+      * intros [ hlt | [ e _ ] ].
+        -- have hlt' : SOrd.lt s s by etransitivity; eauto.
+           now apply SOrd.lt_strorder in hlt'.
+        -- subst; now apply SOrd.lt_strorder in H.
+  - apply IHF.
+  - split.
+    + intros [hlt | [ e hlt ]%andb_prop ]%Bool.orb_prop.
+      * left. rewrite -IHF1 //.
+      * right; split.
+        -- now rewrite -eqbIsEq.
+        -- rewrite -IHF2 //.
+    + intros [ hlt | [ e hlt ] ]; apply Bool.orb_true_intro.
+      * left. now rewrite IHF1.
+      * right; apply andb_true_intro; split.
+        -- rewrite eqbIsEq //.
+        -- rewrite IHF2 //.
+  - apply IHF.
+Qed.
+
+Lemma ltb_form_false :
+  forall (F G : Form),
+    ltb_form F G = false -> F <> G -> ltb_form G F = true.
+Proof.
+  intro F; induction F; intros ? hnlt ne; destruct G; cbn in *; try easy.
+  - have hspec := SOrd.compare_spec p s.
+    destruct (SOrd.compare p s); inversion hspec; cbn in *.
+    + destruct (SOrd.compare s p) eqn:hcomp; try easy.
+      * apply ltb_list_false; auto.
+        -- intros. apply ltb_term_false; auto.
+        -- intro; subst; now apply ne.
+      * subst. now rewrite SSet.XOrdProps.ME.compare_refl in hcomp.
+    + destruct (SOrd.compare s p) eqn:hcomp; try easy.
+    + destruct (SOrd.compare s p) eqn:hcomp; try easy.
+      * apply SSet.Raw.MX.compare_eq in hcomp; subst.
+        inversion hspec. now apply SOrd.lt_strorder in H0.
+      * rewrite SSet.Raw.MX.compare_gt_iff in hcomp.
+        have contra : SOrd.lt s s by etransitivity; eauto.
+        now apply SOrd.lt_strorder in contra.
+  - apply IHF; auto. congruence.
+  - apply Bool.orb_false_elim in hnlt; destruct hnlt as [ne0 h].
+    rewrite Bool.andb_false_iff in h; destruct h as [ne1 | ne1];
+      apply Bool.orb_true_intro.
+    + left. apply IHF1; auto. rewrite EqBool_neq //.
+    + have [hF1 | [ e1 hF2 ] ] : F1 <> G1 \/ (F1 = G1 /\ F2 <> G2).
+      { destruct (F1 == G1); auto.
+        right. split; auto. intro. apply ne; now subst. }
+      * left. apply IHF1; auto.
+      * right. apply andb_true_intro; split.
+        -- rewrite eqbIsEq //.
+        -- apply IHF2; auto.
+  - apply IHF; auto. congruence.
+Qed.
+
+(** Of course, [lt_term] and [lt_form] are both strict orders. *)
+#[global] Instance lt_term_strorder : StrictOrder lt_term.
+Proof.
+  constructor.
+  - intros t; induction t using term_ind; unfold complement; cbn; auto.
+    + apply PeanoNat.Nat.lt_irrefl.
+    + apply SOrd.lt_strorder.
+    + intros [ contra | [_ contra ] ].
+      * now apply SOrd.lt_strorder in contra.
+      * induction l as [|t l' IHl']; auto.
+        cbn in contra. destruct contra as [ contra | [ _ contra ] ].
+        -- now apply Ind.Forall_inv in H.
+        -- apply IHl'; auto. now apply Ind.Forall_tail in H.
+  - intros t0 t1 t2 hlt0 hlt1. generalize dependent t2; generalize dependent t0.
+    induction t1 using term_ind; intros t0 hlt0 t2 hlt1.
+    + destruct t0, t2; auto.
+      * cbn in *. etransitivity; eauto.
+      * cbn in *. inversion hlt0.
+      * cbn in *. inversion hlt0.
+    + destruct t0, t2; auto.
+      * cbn in *. inversion hlt1.
+      * cbn in *. etransitivity; eauto.
+      * cbn in *. inversion hlt0.
+    + destruct t0, t2; auto.
+      * cbn in *. inversion hlt1.
+      * cbn in *. inversion hlt1.
+      * cbn in *. destruct hlt0 as [ hlt0 | [ e0 hltlist0 ] ],
+            hlt1 as [ hlt1 | [ e1 hltlist1 ] ].
+        -- left; etransitivity; eauto.
+        -- rewrite e1 in hlt0. now left.
+        -- rewrite -e0 in hlt1. now left.
+        -- right; split.
+           ++ etransitivity; eauto.
+           ++ clear e0 e1 f s0. generalize dependent l; generalize dependent l1;
+                induction l0 as [|t ts IHts];
+                intros l1 l IHl hltlist hltlist1.
+              ** destruct l1.
+                 --- destruct l; easy.
+                 --- now cbn.
+              ** destruct l1.
+                 --- destruct l; easy.
+                 --- destruct l; try easy.
+                     cbn in *. destruct hltlist as [ hlt1 | [ e1 hlt ] ],
+                         hltlist1 as [ hlt0 | [ e0 hltl1 ] ].
+                     +++ apply Ind.Forall_inv in IHl; left; auto.
+                     +++ left. now rewrite -e0.
+                     +++ left. now rewrite e1.
+                     +++ right; split.
+                         *** etransitivity; eauto.
+                         *** apply IHts with (l := l).
+                             ---- now apply Ind.Forall_tail in IHl.
+                             ---- auto.
+                             ---- auto.
+Qed.
+
+#[global] Instance lt_strorder : StrictOrder lt_form.
+Proof.
+  constructor.
+  - intros F; induction F; unfold complement; cbn; auto.
+    + intros [ contra | [_ contra] ].
+      * now apply SOrd.lt_strorder in contra.
+      * induction l as [|t l' IHl'].
+        -- now cbn in contra.
+        -- cbn in contra; destruct contra.
+           ++ now apply lt_term_strorder in H.
+           ++ destruct H; auto.
+    + intros [contra | [ _ contra ] ]; auto.
+  - intros F G H hlt0 hlt1. generalize dependent H; generalize dependent F.
+    induction G; intros F hlt0 H hlt1.
+    + destruct F; easy.
+    + destruct F, H; try easy.
+      cbn in *. destruct hlt0 as [ hlt0 | [ e0 hltl0 ] ],
+          hlt1 as [ hlt1 | [ e1 hltl1 ] ].
+      * left; etransitivity; eauto.
+      * left. now rewrite -e1.
+      * left. now rewrite e0.
+      * right; split.
+        -- etransitivity; eauto.
+        -- clear e0 e1 p s s0. generalize dependent l; generalize dependent l1;
+             induction l0 as [|t ts IHts];
+             intros l1 l hltlist hltlist1.
+           ++ destruct l1, l; easy.
+           ++ destruct l1, l; try easy.
+              cbn in *. destruct hltlist as [ hlt1 | [ e1 hltl ] ],
+                  hltlist1 as [ hlt0 | [ e0 hltl1 ] ].
+              ** left; etransitivity; eauto.
+              ** left; now rewrite -e0.
+              ** left; now rewrite e1.
+              ** right; split.
+                 --- etransitivity; eauto.
+                 --- eapply IHts; eauto.
+    + destruct F, H; try easy.
+      cbn in *; eapply IHG; eauto.
+    + destruct F, H; try easy.
+      cbn in *. destruct hlt0 as [ hlt1' | [ e1 hlt2 ] ],
+          hlt1 as [ hlt | [ e hlt0 ] ].
+      * left; eapply IHG1; eauto.
+      * left; now rewrite -e.
+      * left; now rewrite e1.
+      * right; split.
+        -- etransitivity; eauto.
+        -- eapply IHG2; eauto.
+    + destruct F, H; try easy.
+      cbn in *; eapply IHG; eauto.
+Qed.
+
+(** We can now give an [OrderedType] structure for formulas. *)
+Module OrderedForm <: OrderedType.
+  Definition t := Form.
+
+  Definition eq : t -> t -> Prop := eq.
+
+  Lemma eq_equiv : Equivalence eq.
+  Proof. typeclasses eauto. Qed.
+
+  Definition lt := lt_form.
+
+  Lemma lt_strorder : StrictOrder lt.
+  Proof. ltac:(typeclasses eauto). Qed.
+
+  #[global] Instance lt_compat : Proper (eq ==> eq ==> iff) lt.
+  Proof. intros F G ->; cbn. intros F H ->; cbn. reflexivity. Qed.
+
+  Definition compare (F G : Form) : comparison :=
+    if eqb F G then Eq
+    else if ltb_form F G then Lt
+         else Gt.
+
+  Lemma compare_spec :
+    forall (F G : Form), CompareSpec (F = G) (lt F G) (lt G F) (compare F G).
+  Proof.
+    intros ??. destruct (F == G).
+    - subst. unfold compare. rewrite EqBool_refl. now constructor.
+    - unfold compare. rewrite EqBool_neq in n; rewrite n.
+      destruct (ltb_form F G) eqn:hlt.
+      + constructor. unfold lt; rewrite -ltb_form_lt_form //.
+      + constructor. unfold lt.
+        rewrite -ltb_form_lt_form.
+        apply ltb_form_false; auto.
+        rewrite EqBool_neq //.
+  Qed.
+
+  Definition eq_dec (F G : Form) : { F = G } + { F <> G }.
+  Proof. apply eq_dec_from_eq_bool; typeclasses eauto. Qed.
+End OrderedForm.
+
+(** Which means that we can give computational sets of formulas. *)
+Module FSet := MSetAVL.Make OrderedForm.
+
