shell.nix
@@ -1,11 +1,32 @@
-{ pkgs ? import ./devtools/nixpkgs.nix {} }:
+{ lib
+, pkgs ? import ./devtools/nixpkgs.nix {}
+, withDoc ? true
+, withExtraction ? true
+, withOCamlDev ? true }:
 
 pkgs.mkShell {
   nativeBuildInputs = with pkgs.buildPackages; [
+    # Base packages
     gnumake
+  ] ++ [
+    # Packages used by the Rocq library
     rocq-core
     rocqPackages.stdlib
     ocamlPackages.findlib
+  ] ++ (lib.optionals withDoc [
+    # Packages for building the documentation
     pandoc
-  ];
+  ]) ++ (lib.optionals withExtraction [
+    # Packages for building the extraction
+    ocaml
+    dune_3
+  ]) ++ (lib.optionals withOCamlDev [
+    # Packages for developing the non-critical OCaml code
+    pkgs.ocamlPackages.ocaml-lsp
+    pkgs.ocamlPackages.ocamlformat
+    pkgs.ocamlPackages.ocp-indent
+    pkgs.ocamlPackages.ocp-index
+    pkgs.ocamlPackages.merlin
+    pkgs.ocamlPackages.menhir
+  ]);
 }
